sprop_universe/cwf.v
@@ -1,0 +1,550 @@
+(* ************************************* *)
+(* A Universe for Proof-Relevant Setoids *)
+(* ************************************* *)
+
+(* This file contains the definition of our setoid model as a CwF *)
+
+Set Universe Polymorphism.
+Set Primitive Projections.
+Require Import utils.
+Require Import univ0 univ0_lemmas.
+Require Import univ1 univ1_lemmas.
+
+(* We define our model as a CwF. The type of contexts is U1. *)
+
+Definition Con := U1.
+
+Definition arr1 (A B : U1) : U1 := Pi1 A (fun _ => B) (fun _ _ _ => reflU1 B).
+Definition Sub (Δ Γ : Con) := El1 (arr1 Δ Γ).
+
+(* Identity substitution *)
+
+Definition idSub (Γ : Con) : Sub Γ Γ.
+Proof.
+  unshelve econstructor.
+  - exact (fun x => x).
+  - intros. exact ae.
+Defined.
+
+(* Substitution composition *)
+
+Definition compSub {Γ Δ Ξ : Con} (σ : Sub Δ Γ) (τ : Sub Ξ Δ) : Sub Ξ Γ.
+Proof.
+  unshelve econstructor.
+  - exact (fun x => fsts σ (fsts τ x)).
+  - intros. refine (snds σ (fsts τ a0) (fsts τ a1) _).
+    exact (snds τ a0 a1 ae).
+Defined.
+Notation "σ ∘ τ" := (compSub σ τ) (at level 60, right associativity).
+
+(* Composition is definitionally associative and unital *)
+
+Lemma compAssoc {Γ Δ Ξ Ξ' : Con} (σ : Sub Δ Γ) (τ : Sub Ξ Δ) (τ' : Sub Ξ' Ξ) : (σ ∘ τ) ∘ τ' = σ ∘ (τ ∘ τ').
+Proof.
+  reflexivity.
+Qed.
+
+Lemma compIdLeft {Γ Δ : Con} (σ : Sub Δ Γ) : (idSub Γ) ∘ σ = σ.
+Proof.
+  reflexivity.
+Qed.
+
+Lemma compIdRight {Γ Δ : Con} (σ : Sub Δ Γ) : σ ∘ (idSub Δ) = σ.
+Proof.
+  reflexivity.
+Qed.
+
+(* Dependent types *)
+
+Definition Ty (Γ : Con) := El1 (arr1 Γ U01).
+
+(* Substitution/reindexing of types *)
+
+Definition tySubst {Γ Δ : Con} (A : Ty Γ) (σ : Sub Δ Γ) : Ty Δ := A ∘ σ.
+
+Notation "A [ σ ]T" := (tySubst A σ) (at level 30).
+
+(* Substitution is definitionally functorial *)
+
+Lemma substId {Γ : Con} (A : Ty Γ) : A [ idSub Γ ]T = A.
+Proof.
+  reflexivity.
+Qed.
+
+Lemma substComp {Γ Δ Ξ : Con} (A : Ty Γ) (σ : Sub Δ Γ) (τ : Sub Ξ Δ) : A [ σ ∘ τ ]T = A [ σ ]T [ τ ]T.
+Proof.
+  reflexivity.
+Qed.
+
+(* Terms *)
+
+Definition Tm (Γ : Con) (A : Ty Γ) := El1 (Pi1 Γ (fun γ => emb1 (fsts A γ)) (snds A)).
+
+(* Substitution/reindexing of terms *)
+
+Definition tmSubst {Γ Δ : Con} {A : Ty Γ} (t : Tm Γ A) (σ : Sub Δ Γ) : Tm Δ (A [σ]T).
+Proof.
+  unshelve econstructor.
+  - exact (fun δ => fsts t (fsts σ δ)).
+  - refine (fun δ0 δ1 δe => snds t (fsts σ δ0) (fsts σ δ1) (snds σ δ0 δ1 δe)).
+Defined.
+
+Notation "a [ σ ]t" := (tmSubst a σ) (at level 30).
+
+(* Substitution is definitionally functorial *)
+
+Lemma substIdTm {Γ : Con} (A : Ty Γ) (a : Tm Γ A) : a [ idSub Γ ]t = a.
+Proof.
+  reflexivity.
+Qed.
+
+Lemma substCompTm {Γ Δ Ξ : Con} (A : Ty Γ) (a : Tm Γ A) (σ : Sub Δ Γ) (τ : Sub Ξ Δ) : a [ σ ∘ τ ]t = a [ σ ]t [ τ ]t.
+Proof.
+  reflexivity.
+Qed.
+
+(* Context extension with weakening, variable (p and q in CwF notations) and substitution extension *)
+
+Definition ConExt (Γ : Con) (A : Ty Γ) : Con := Sigma1 Γ (fun γ => emb1 (fsts A γ)) (snds A).
+
+Notation "Γ ▹ A" := (ConExt Γ A) (at level 50, left associativity).
+
+Definition wk {Γ : Con} (A : Ty Γ) : Sub (Γ ▹ A) Γ.
+Proof.
+  unshelve econstructor.
+  - exact (fun x => fst x).
+  - exact (fun x0 x1 xe => andleft xe).
+Defined.
+
+Definition var0 {Γ : Con} (A : Ty Γ) : Tm (Γ ▹ A) (A [wk A]T).
+Proof.
+  unshelve econstructor.
+  - exact (fun x => snd x).
+  - exact (fun x0 x1 xe => andright xe).
+Defined.
+
+Definition subExt {Γ Δ : Con} (A : Ty Γ) (σ : Sub Δ Γ) (a : Tm Δ (A [σ]T)) : Sub Δ (Γ ▹ A).
+Proof.
+  unshelve econstructor.
+  - exact (fun δ => mkPair (fsts σ δ) (fsts a δ)).
+  - refine (fun δ0 δ1 δe => mkAndEx (snds σ δ0 δ1 δe) (snds a δ0 δ1 δe)).
+Defined.
+
+Notation "⟨ σ , a ⟩" := (subExt _ σ a).
+
+(* β and η laws for substitutions are definitional *)
+
+Lemma subExtβ1 {Γ Δ : Con} (A : Ty Γ) (σ : Sub Δ Γ) (a : Tm Δ (A [σ]T)) : (wk A) ∘ ⟨ σ , a ⟩ = σ.
+Proof.
+  reflexivity.
+Qed.
+
+Lemma subExtβ2 {Γ Δ : Con} (A : Ty Γ) (σ : Sub Δ Γ) (a : Tm Δ (A [σ]T)) : (var0 A)[⟨ σ , a ⟩]t = a.
+Proof.
+  reflexivity.
+Qed.
+
+Lemma subExtη {Γ Δ : Con} (A : Ty Γ) (σ : Sub Δ (Γ ▹ A)) : σ = ⟨ (wk A) ∘ σ , (var0 A)[σ]t ⟩.
+Proof.
+  reflexivity.
+Qed.
+
+(* Thus we have a CwF in which all the equations are definitional.
+   Now it remains to show that this CwF supports all the type formers of MLTT. *)
+
+(* But first, some utilities for substitutions *)
+
+Definition lift {Γ Δ : Con} (σ : Sub Δ Γ) (A : Ty Γ) : Sub (Δ ▹ A [σ]T) (Γ ▹ A).
+Proof.
+  unshelve econstructor.
+  - exact (fun x => mkPair (fsts σ (fst x)) (snd x)).
+  - unshelve refine (fun x0 x1 xe => mkAndEx (snds σ (fst x0) (fst x1) (andleft xe)) (andright xe)).
+Defined.
+
+Definition sgSub {Γ : Con} {A : Ty Γ} (t : Tm Γ A) : Sub Γ (Γ ▹ A) := ⟨ idSub Γ , t ⟩.
+
+(* Dependent products *)
+
+Definition Π {Γ : Con} (A : Ty Γ) (B : Ty (Γ ▹ A)) : Ty Γ.
+Proof.
+  unshelve econstructor.
+  - exact (fun γ => Pi0 (fsts A γ) (fun a => fsts B (mkPair γ a))
+                        (fun a0 a1 ae => snds B (mkPair γ a0) (mkPair γ a1) (mkAndEx (refl1 Γ γ) ae))).
+  - exact (fun γ0 γ1 γe => sand_intro (snds A γ0 γ1 γe)
+                                      (fun a0 a1 ae => snds B (mkPair γ0 a0) (mkPair γ1 a1) (mkAndEx γe ae))).
+Defined.
+
+Lemma substΠ {Γ Δ : Con} (A : Ty Γ) (B : Ty (Γ ▹ A)) (σ : Sub Δ Γ) : (Π A B) [σ]T = Π (A [σ]T) (B [lift σ A]T).
+Proof.
+  reflexivity.
+Qed.
+
+(* Lambda abstraction *)
+
+Definition lam {Γ : Con} (A : Ty Γ) (B : Ty (Γ ▹ A)) (t : Tm (Γ ▹ A) B) : Tm Γ (Π A B).
+Proof.
+  unshelve econstructor.
+  - intro γ. unshelve econstructor.
+    + exact (fun a => fsts t (mkPair γ a)).
+    + unshelve refine (fun a0 a1 ae => snds t (mkPair γ a0) (mkPair γ a1) (mkAndEx (refl1 Γ γ) ae)).
+  - exact (fun γ0 γ1 γe a0 a1 ae => snds t (mkPair γ0 a0) (mkPair γ1 a1) (mkAndEx γe ae)).
+Defined.
+
+Lemma substLam {Γ Δ : Con} (A : Ty Γ) (B : Ty (Γ ▹ A)) (t : Tm (Γ ▹ A) B) (σ : Sub Δ Γ) :
+  (lam A B t) [σ]t = lam (A [σ]T) (B [lift σ A]T) (t [lift σ A]t).
+Proof.
+  reflexivity.
+Qed.
+
+(* Function application *)
+
+Definition app {Γ : Con} (A : Ty Γ) (B : Ty (Γ ▹ A)) (t : Tm Γ (Π A B)) (u : Tm Γ A) : Tm Γ (B [sgSub u]T).
+Proof.
+  unshelve econstructor.
+  - exact (fun γ => fsts (fsts t γ) (fsts u γ)).
+  - exact (fun γ0 γ1 γe => snds t γ0 γ1 γe (fsts u γ0) (fsts u γ1) (snds u γ0 γ1 γe)).
+Defined.
+
+Lemma substApp {Γ Δ : Con} (A : Ty Γ) (B : Ty (Γ ▹ A)) (t : Tm Γ (Π A B)) (u : Tm Γ A) (σ : Sub Δ Γ) :
+  (app A B t u) [σ]t = app (A [σ]T) (B [lift σ A]T) (t [σ]t) (u [σ]t).
+Proof.
+  reflexivity.
+Qed.
+
+(* β and η laws for functions are definitional *)
+
+Lemma Πβ {Γ : Con} (A : Ty Γ) (B : Ty (Γ ▹ A)) (t : Tm (Γ ▹ A) B) (u : Tm Γ A) : app A B (lam A B t) u = t [sgSub u]t.
+Proof.
+  reflexivity.
+Qed.
+
+Lemma Πη {Γ : Con} (A : Ty Γ) (B : Ty (Γ ▹ A)) (t : Tm Γ (Π A B)) : t = lam A B (app (A [wk A]T) (B [lift (wk A) A]T) (t [wk A]t) (var0 A)).
+Proof.
+  reflexivity.
+Qed.
+
+(* Nondependent function type *)
+
+Definition arr {Γ : Con} (A : Ty Γ) (B : Ty Γ) : Ty Γ.
+Proof.
+  unshelve econstructor.
+  - exact (fun γ => Pi0 (fsts A γ) (fun _ => fsts B γ)
+                        (fun _ _ _ => reflU0 (fsts B γ))).
+  - exact (fun γ0 γ1 γe => sand_intro (snds A γ0 γ1 γe)
+                                      (fun _ _ _ => snds B γ0 γ1 γe)).
+Defined.
+
+Lemma substArr {Γ Δ : Con} (A : Ty Γ) (B : Ty Γ) (σ : Sub Δ Γ) : (arr A B) [σ]T = arr (A [σ]T) (B [σ]T).
+Proof.
+  reflexivity.
+Qed.
+
+Definition app' {Γ : Con} (A : Ty Γ) (B : Ty Γ) (t : Tm Γ (arr A B)) (u : Tm Γ A) : Tm Γ B.
+Proof.
+  unshelve econstructor.
+  - exact (fun γ => fsts (fsts t γ) (fsts u γ)).
+  - exact (fun γ0 γ1 γe => snds t γ0 γ1 γe (fsts u γ0) (fsts u γ1) (snds u γ0 γ1 γe)).
+Defined.
+
+Lemma substApp' {Γ Δ : Con} (A : Ty Γ) (B : Ty Γ) (t : Tm Γ (arr A B)) (u : Tm Γ A) (σ : Sub Δ Γ) :
+  (app' A B t u) [σ]t = app' (A [σ]T) (B [σ]T) (t [σ]t) (u [σ]t).
+Proof.
+  reflexivity.
+Qed.
+
+(* Σ-types *)
+
+Definition Σ {Γ : Con} (A : Ty Γ) (B : Ty (Γ ▹ A)) : Ty Γ.
+Proof.
+  unshelve econstructor.
+  - exact (fun γ => Sigma0 (fsts A γ) (fun a => fsts B (mkPair γ a))
+                           (fun a0 a1 ae => snds B (mkPair γ a0) (mkPair γ a1) (mkAndEx (refl1 Γ γ) ae))).
+  - exact (fun γ0 γ1 γe => sand_intro (snds A γ0 γ1 γe)
+                                      (fun a0 a1 ae => snds B (mkPair γ0 a0) (mkPair γ1 a1) (mkAndEx γe ae))).
+Defined.
+
+Lemma substΣ {Γ Δ : Con} (A : Ty Γ) (B : Ty (Γ ▹ A)) (σ : Sub Δ Γ) : (Σ A B) [σ]T = Σ (A [σ]T) (B [lift σ A]T).
+Proof.
+  reflexivity.
+Qed.
+
+(* Pair constructor *)
+
+Definition pair {Γ : Con} (A : Ty Γ) (B : Ty (Γ ▹ A)) (t : Tm Γ A) (u : Tm Γ (B [sgSub t]T)) : Tm Γ (Σ A B).
+Proof.
+  unshelve econstructor.
+  - intro γ. unshelve refine (mkPair _ _). exact (fsts t γ). exact (fsts u γ). (* weird universe inconsistency if I give the term directly *)
+  - intros γ0 γ1 γe. unshelve refine (mkAndEx (snds t γ0 γ1 γe) (snds u γ0 γ1 γe)).
+Defined.
+
+Lemma substPair {Γ Δ : Con} (A : Ty Γ) (B : Ty (Γ ▹ A)) (t : Tm Γ A) (u : Tm Γ (B [sgSub t]T)) (σ : Sub Δ Γ) :
+  (pair A B t u) [σ]t = pair (A [σ]T) (B [lift σ A]T) (t [σ]t) (u [σ]t).
+Proof.
+  reflexivity.
+Qed.
+
+(* First projection *)
+
+Definition proj1 {Γ : Con} (A : Ty Γ) (B : Ty (Γ ▹ A)) (t : Tm Γ (Σ A B)) : Tm Γ A.
+Proof.
+  unshelve econstructor.
+  - exact (fun γ => fst (fsts t γ)).
+  - exact (fun γ0 γ1 γe => andleft (snds t γ0 γ1 γe)).
+Defined.
+
+Lemma substProj1 {Γ Δ : Con} (A : Ty Γ) (B : Ty (Γ ▹ A)) (t : Tm Γ (Σ A B)) (σ : Sub Δ Γ) :
+  (proj1 A B t) [σ]t = proj1 (A [σ]T) (B [lift σ A]T) (t [σ]t).
+Proof.
+  reflexivity.
+Qed.
+
+(* Second projection *)
+
+Definition proj2 {Γ : Con} (A : Ty Γ) (B : Ty (Γ ▹ A)) (t : Tm Γ (Σ A B)) : Tm Γ (B [sgSub (proj1 A B t)]T).
+Proof.
+  unshelve econstructor.
+  - exact (fun γ => snd (fsts t γ)).
+  - exact (fun γ0 γ1 γe => andright (snds t γ0 γ1 γe)).
+Defined.
+
+Lemma substProj2 {Γ Δ : Con} (A : Ty Γ) (B : Ty (Γ ▹ A)) (t : Tm Γ (Σ A B)) (σ : Sub Δ Γ) :
+  (proj2 A B t) [σ]t = proj2 (A [σ]T) (B [lift σ A]T) (t [σ]t).
+Proof.
+  reflexivity.
+Qed.
+
+(* β and η laws for pairs are definitional *)
+
+Lemma Σβ1 {Γ : Con} (A : Ty Γ) (B : Ty (Γ ▹ A)) (t : Tm Γ A) (u : Tm Γ (B [sgSub t]T)) :
+  proj1 A B (pair A B t u) = t.
+Proof.
+  reflexivity.
+Qed.
+
+Lemma Σβ2 {Γ : Con} (A : Ty Γ) (B : Ty (Γ ▹ A)) (t : Tm Γ A) (u : Tm Γ (B [sgSub t]T)) :
+  proj2 A B (pair A B t u) = u.
+Proof.
+  reflexivity.
+Qed.
+
+Lemma Ση {Γ : Con} (A : Ty Γ) (B : Ty (Γ ▹ A)) (t : Tm Γ (Σ A B)) :
+  t = pair A B (proj1 A B t) (proj2 A B t).
+Proof.
+  reflexivity.
+Qed.
+
+(* Natural numbers *)
+
+Definition ℕ (Γ : Con) : Ty Γ.
+Proof.
+  unshelve econstructor.
+  - exact (fun _ => nat0).
+  - exact (fun _ _ _ => stt).
+Defined.
+
+Lemma substℕ {Γ Δ : Con} (σ : Sub Δ Γ) : (ℕ Γ) [σ]T = ℕ Δ.
+Proof.
+  reflexivity.
+Qed.
+
+(* zero *)
+
+Definition ℕz (Γ : Con) : Tm Γ (ℕ Γ).
+Proof.
+  unshelve econstructor.
+  - exact (fun _ => zero).
+  - exact (fun _ _ _ => eqzero).
+Defined.
+
+Lemma substℕz {Γ Δ : Con} (σ : Sub Δ Γ) : (ℕz Γ) [σ]t = ℕz Δ.
+Proof.
+  reflexivity.
+Qed.
+
+(* successor *)
+
+Definition ℕS (Γ : Con) (n : Tm Γ (ℕ Γ)) : Tm Γ (ℕ Γ).
+Proof.
+  unshelve econstructor.
+  - exact (fun γ => suc (fsts n γ)).
+  - exact (fun γ0 γ1 γe => eqsuc (fsts n γ0) (fsts n γ1) (snds n γ0 γ1 γe)).
+Defined.
+
+Lemma substℕS {Γ Δ : Con} (n : Tm Γ (ℕ Γ)) (σ : Sub Δ Γ) : (ℕS Γ n) [σ]t = ℕS Δ (n [σ]t).
+Proof.
+  reflexivity.
+Qed.
+
+(* eliminator *)
+
+Definition ℕemb (n : nat) (Γ : Con) : Tm Γ (ℕ Γ).
+Proof.
+  unshelve econstructor.
+  - exact (fun _ => n).
+  - exact (fun _ _ _ => nateq_refl n).
+Defined.
+
+Definition ℕrec (Γ : Con) (P : Ty (Γ ▹ (ℕ Γ))) (pZ : Tm Γ (P [sgSub (ℕz Γ)]T))
+  (pS : Tm (Γ ▹ (ℕ Γ)) (arr P (P [(subExt (ℕ Γ) (wk (ℕ Γ)) (ℕS (Γ ▹ (ℕ Γ)) (var0 (ℕ Γ))))]T)))
+  (n : Tm Γ (ℕ Γ)) : Tm Γ (P [sgSub n]T).
+Proof.
+  unshelve econstructor.
+  - intro γ. refine (nat_rect (fun n => El0 (fsts (P [@sgSub Γ (ℕ Γ) (ℕemb n Γ)]T) γ)) _ _ (fsts n γ)).
+    + exact (fsts pZ γ).
+    + intros m IH. exact (fsts (fsts pS (mkPair γ m)) IH).
+  - intros γ0 γ1 γe.
+    refine (nateq_sind (fun n0 n1 ne => eq0 _ _
+        (nat_rect (fun n => El0 (fsts (P [@sgSub Γ (ℕ Γ) (ℕemb n Γ)]T) γ0)) (fsts pZ γ0) (fun m IH => fsts (fsts pS (mkPair γ0 m)) IH) n0)
+        (nat_rect (fun n => El0 (fsts (P [@sgSub Γ (ℕ Γ) (ℕemb n Γ)]T) γ1)) (fsts pZ γ1) (fun m IH => fsts (fsts pS (mkPair γ1 m)) IH) n1))
+      _ _ (fsts n γ0) (fsts n γ1) (snds n γ0 γ1 γe)).
+    + exact (snds pZ γ0 γ1 γe).
+    + intros m0 m1 me IH. refine (snds pS (mkPair γ0 m0) (mkPair γ1 m1) (mkAndEx γe me) _ _ IH).
+Defined.
+
+Lemma substℕrec (Γ Δ : Con) (P : Ty (Γ ▹ (ℕ Γ))) (pZ : Tm Γ (P [sgSub (ℕz Γ)]T))
+  (pS : Tm (Γ ▹ (ℕ Γ)) (arr P (P [(subExt (ℕ Γ) (wk (ℕ Γ)) (ℕS (Γ ▹ (ℕ Γ)) (var0 (ℕ Γ))))]T)))
+  (n : Tm Γ (ℕ Γ)) (σ : Sub Δ Γ) :
+  (ℕrec Γ P pZ pS n) [σ]t = ℕrec Δ (P [lift σ (ℕ Γ)]T) (pZ [σ]t) (pS [lift σ (ℕ Γ)]t) (n [σ]t).
+Proof.
+  reflexivity.
+Qed.
+
+(* β laws for natural numbers are definitional *)
+
+Lemma ℕβ1 (Γ : Con) (P : Ty (Γ ▹ (ℕ Γ))) (pZ : Tm Γ (P [sgSub (ℕz Γ)]T))
+  (pS : Tm (Γ ▹ (ℕ Γ)) (arr P (P [(subExt (ℕ Γ) (wk (ℕ Γ)) (ℕS (Γ ▹ (ℕ Γ)) (var0 (ℕ Γ))))]T))) :
+  ℕrec Γ P pZ pS (ℕz Γ) = pZ.
+Proof.
+  reflexivity.
+Qed.
+
+Lemma ℕβ2 (Γ : Con) (P : Ty (Γ ▹ (ℕ Γ))) (pZ : Tm Γ (P [sgSub (ℕz Γ)]T))
+  (pS : Tm (Γ ▹ (ℕ Γ)) (arr P (P [(subExt (ℕ Γ) (wk (ℕ Γ)) (ℕS (Γ ▹ (ℕ Γ)) (var0 (ℕ Γ))))]T))) (n : Tm Γ (ℕ Γ)) :
+  ℕrec Γ P pZ pS (ℕS Γ n) = app' (P [sgSub n]T) (P [sgSub (ℕS Γ n)]T) (pS [sgSub n]t) (ℕrec Γ P pZ pS n).
+Proof.
+  reflexivity.
+Qed.
+
+(* Universe of propositions *)
+
+Definition Ω (Γ : Con) : Ty Γ.
+Proof.
+  unshelve econstructor.
+  - exact (fun _ => SProp0).
+  - exact (fun _ _ _ => stt).
+Defined.
+
+Lemma substΩ {Γ Δ : Con} (σ : Sub Δ Γ) : (Ω Γ) [σ]T = Ω Δ.
+Proof.
+  reflexivity.
+Qed.
+
+(* Type of elements of a proposition *)
+
+Definition Prf {Γ : Con} (P : Tm Γ (Ω Γ)) : Ty Γ.
+Proof.
+  unshelve econstructor.
+  - exact (fun γ => emb0 (fsts P γ)).
+  - exact (snds P).
+Defined.
+
+Lemma substPrf {Γ Δ : Con} (P : Tm Γ (Ω Γ)) (σ : Sub Δ Γ) : (Prf P) [σ]T = Prf (P [σ]t).
+Proof.
+  reflexivity.
+Qed.
+
+(* Propositions SHOULD satisfy definitional proof irrelevance. However, that requires η for the embedding of SProp into Type
+   (for instance, a record with one SProp field would do the trick, but these do not support η in Rocq at the moment) *)
+
+Lemma prfIrr {Γ : Con} (P : Tm Γ (Ω Γ)) (p q : Tm Γ (Prf P)) : p = q.
+Proof.
+  Fail reflexivity.
+Abort.
+
+(* False proposition *)
+
+Definition false (Γ : Con) : Tm Γ (Ω Γ).
+Proof.
+  unshelve econstructor.
+  - exact (fun γ => sFalse).
+  - exact (fun γ0 γ1 γe => sand_intro (fun x => x) (fun x => x)).
+Defined.
+
+Lemma substFalse {Γ Δ : Con} (σ : Sub Δ Γ) : (false Γ) [σ]t = false Δ.
+Proof.
+  reflexivity.
+Qed.
+
+(* Large elimination of False *)
+
+Definition efq {Γ : Con} (A : Ty Γ) (abs : Tm Γ (Prf (false Γ))) : Tm Γ A.
+Proof.
+  unshelve econstructor.
+  - exact (fun γ => sFalse_rect (fun _ => El0 (fsts A γ)) (to_set_esc sFalse (fsts abs γ))).
+  - refine (fun γ0 γ1 γe => _). destruct (fsts abs γ0). destruct a.
+Defined.
+
+Lemma substEfq {Γ Δ : Con} (A : Ty Γ) (abs : Tm Γ (Prf (false Γ))) (σ : Sub Δ Γ) :
+  (efq A abs) [σ]t = efq (A [σ]T) (abs[σ]t).
+Proof.
+  reflexivity.
+Qed.
+
+(* Impredicative quantification *)
+
+Definition for_all {Γ : Con} (A : Ty Γ) (P : Tm (Γ ▹ A) (Ω (Γ ▹ A))) : Tm Γ (Ω Γ).
+Proof.
+  unshelve econstructor.
+  - exact (fun γ => forall (a : El0 (fsts A γ)), fsts P (mkPair γ a)).
+  - intros γ0 γ1 γe. econstructor.
+    + intros H a1. set (a0 := cast0 (fsts A γ1) (fsts A γ0) (symU0 _ _ (snds A γ0 γ1 γe)) a1).
+      pose proof (cast0_eq (fsts A γ1) (fsts A γ0) (symU0 _ _ (snds A γ0 γ1 γe)) a1) as ae. change (eq0 _ _ a1 a0) in ae.
+      pose proof (snds P (mkPair γ0 a0) (mkPair γ1 a1) (mkAndEx γe (sym0 _ _ ae))) as Pe.
+      change (sand ((fsts P (mkPair γ0 a0)) -> (fsts P (mkPair γ1 a1))) ((fsts P (mkPair γ1 a1)) -> (fsts P (mkPair γ0 a0)))) in Pe.
+      exact (sand_fst Pe (H a0)).
+    + intros H a0. set (a1 := cast0 (fsts A γ0) (fsts A γ1) (snds A γ0 γ1 γe) a0).
+      pose proof (cast0_eq (fsts A γ0) (fsts A γ1) (snds A γ0 γ1 γe) a0) as ae. change (eq0 _ _ a0 a1) in ae.
+      pose proof (snds P (mkPair γ0 a0) (mkPair γ1 a1) (mkAndEx γe ae)) as Pe.
+      change (sand ((fsts P (mkPair γ0 a0)) -> (fsts P (mkPair γ1 a1))) ((fsts P (mkPair γ1 a1)) -> (fsts P (mkPair γ0 a0)))) in Pe.
+      exact (sand_snd Pe (H a1)).
+Defined.
+
+Lemma substForall {Γ Δ : Con} (A : Ty Γ) (P : Tm (Γ ▹ A) (Ω (Γ ▹ A))) (σ : Sub Δ Γ) :
+  (for_all A P) [σ]t = for_all (A [σ]T) (P [lift σ A]t).
+Proof.
+  reflexivity.
+Qed.
+
+(* Introduction for impredicative forall *)
+
+Definition forall_lam {Γ : Con} (A : Ty Γ) (P : Tm (Γ ▹ A) (Ω (Γ ▹ A))) (t : Tm (Γ ▹ A) (Prf P)) : Tm Γ (Prf (for_all A P)).
+Proof.
+  unshelve econstructor.
+  - exact (fun γ => to_set_intro (fsts (for_all A P) γ) (fun a => to_set_esc _ (fsts t (mkPair γ a)))).
+  - intros γ0 γ1 γe. exact stt.
+Defined.
+
+Lemma substForall_lam {Γ Δ : Con} (A : Ty Γ) (P : Tm (Γ ▹ A) (Ω (Γ ▹ A))) (t : Tm (Γ ▹ A) (Prf P)) (σ : Sub Δ Γ) :
+  (forall_lam A P t) [σ]t = forall_lam (A [σ]T) (P [lift σ A]t) (t [lift σ A]t).
+Proof.
+  reflexivity.
+Qed.
+
+(* Elimination for impredicative forall *)
+
+Definition forall_app {Γ : Con} (A : Ty Γ) (P : Tm (Γ ▹ A) (Ω (Γ ▹ A))) (t : Tm Γ (Prf (for_all A P))) (u : Tm Γ A) :
+  Tm Γ (Prf (P [sgSub u]t)).
+Proof.
+  unshelve econstructor.
+  - refine (fun γ => to_set_intro _ (to_set_esc _ (fsts t γ) (fsts u γ))).
+  - intros γ0 γ1 γe. exact stt.
+Defined.
+
+Lemma substForall_app {Γ Δ : Con} (A : Ty Γ) (P : Tm (Γ ▹ A) (Ω (Γ ▹ A))) (t : Tm Γ (Prf (for_all A P))) (u : Tm Γ A) (σ : Sub Δ Γ) :
+  (forall_app A P t u) [σ]t = forall_app (A [σ]T) (P [lift σ A]t) (t [σ]t) (u [σ]t).
+Proof.
+  reflexivity.
+Qed.
+
+(* TODO: Observational equality with cast, W types and quotients.
+         See model.v for a somewhat less careful version. *)
